Fp/ExtraTheorems.lean
@@ -7,8 +7,6 @@ import Fp.Rounding
 
 -- Helpers
 
-def twoE5M2 : PackedFloat 5 2 := PackedFloat.ofBits _ _ 0b01000000
-
 /-- Doubles the given floating point number, rounding to nearest if applicable. -/
 def doubleRNE (a : PackedFloat e s) : PackedFloat e s :=
   if a.isNaN then PackedFloat.getNaN _ _
@@ -30,22 +28,50 @@ theorem add_eq_mul_two (a : PackedFloat 5 2) (m : RoundingMode)
     -BitVec.shiftLeft_eq', -BitVec.ushiftRight_eq']
   bv_decide
 
-theorem doubleRNE_eq_times_two (a : PackedFloat 5 2)
+theorem doubleRNE_eq_mul_two (a : PackedFloat 5 2)
   : doubleRNE a = mul twoE5M2 a .RNE := by
   apply PackedFloat.inj
   simp [doubleRNE, mul, round, twoE5M2, BitVec.cons,
     -BitVec.shiftLeft_eq', -BitVec.ushiftRight_eq']
   bv_decide
 
+theorem add_neg_self_isZero_or_isNaN (a : PackedFloat 5 2) (m : RoundingMode)
+  : (add (by omega) a (neg a) m).isZero ∨ (add (by omega) a (neg a) m).isNaN := by
+  simp [add, e_add, f_add, neg, round, PackedFloat.toEFixed,
+    -BitVec.shiftLeft_eq', -BitVec.ushiftRight_eq']
+  bv_decide
+
+theorem e_add_monotone (m : RoundingMode) (a b c : EFixedPoint 34 16)
+  (hc : c.state = .Number)
+  : e_le a b → e_le (e_add m a c) (e_add m b c) := by
+  simp_all [e_add, f_add]
+  bv_decide
+
+theorem add_monotone (a b c : PackedFloat 5 2) (m : RoundingMode) (hc : c.isNormOrSubnorm)
+  : le a b → le (add (by omega) a c m) (add (by omega) b c m) := by
+  intro h
+  apply le_of_e_le
+  have hc' : (c.toEFixed (by omega)).state = .Number :=
+    PackedFloat.isNumber_of_isNormOrSubnorm c hc
+  apply e_add_monotone _ _ _ _ hc'
+  exact e_le_of_le _ _ h
+
 theorem sterbenz (a b : PackedFloat 5 2)
-  (hc : a ≠ b)
   (h : le a (doubleRNE b) ∧ le b (doubleRNE a))
-  : add (by omega) a (neg b) .RTN = add (by omega) a (neg b) .RTP
+  : isExactFloat 5 2 (e_add .RTZ (a.toEFixed (by omega)) ((neg b).toEFixed (by omega)))
   := by
-    apply PackedFloat.inj
-    simp [le, doubleRNE] at h
-    simp [← PackedFloat.injEq] at hc
-    simp [add, e_add, f_add, neg, round,
-      PackedFloat.toEFixed,
-      -BitVec.shiftLeft_eq', -BitVec.ushiftRight_eq']
-    bv_decide
+  simp [le, doubleRNE] at h
+  simp [e_add, f_add, neg, round, isExactFloat,
+    PackedFloat.toEFixed,
+    -BitVec.shiftLeft_eq', -BitVec.ushiftRight_eq']
+  bv_decide
+
+theorem sterbenzFP16 (a b : PackedFloat 5 10)
+  (h : le a (doubleRNE b) ∧ le b (doubleRNE a))
+  : isExactFloat 5 10 (e_add .RTZ (a.toEFixed (by omega)) ((neg b).toEFixed (by omega)))
+  := by
+  simp [le, doubleRNE] at h
+  simp [e_add, f_add, neg, round, isExactFloat,
+    PackedFloat.toEFixed,
+    -BitVec.shiftLeft_eq', -BitVec.ushiftRight_eq']
+  bv_decide
